PAC_Checker2/LPAC_Checker_Synthesis.thy
@@ -7,7 +7,6 @@ theory LPAC_Checker_Synthesis
   imports
     LPAC_Checker
     LPAC_Version
-    LPAC_Steps_Refine
     PAC_Checker_LLVM.More_Loops
     PAC_Checker_LLVM.PAC_Checker_Relation
     PAC_Checker_LLVM.PAC_Checker_Synthesis
@@ -17,89 +16,309 @@ hide_const (open) PAC_Checker.PAC_checker_l
 
 section \<open>Code Synthesis of the Complete Checker\<close>
 
-definition check_linear_combi_l_pre_err_impl :: \<open>uint64 \<Rightarrow> bool \<Rightarrow> bool \<Rightarrow> bool \<Rightarrow> string\<close> where
+(* For now we ignore printing - we will have to figure this out at some point though
+definition check_linear_combi_l_pre_err_impl 
+  :: \<open>nat \<Rightarrow> bool \<Rightarrow> bool \<Rightarrow> bool \<Rightarrow> string\<close> where
   \<open>check_linear_combi_l_pre_err_impl i adom emptyl ivars =
-  ''Precondition for '%' failed '' @ show (nat_of_uint64 i) @
+  ''Precondition for '%' failed '' @ show i @
   ''(already in domain: '' @ show adom @
   ''; empty CL'' @ show emptyl @
   ''; new vars: '' @ show ivars @ '')''\<close>
-
-abbreviation comp4 (infixl "oooo" 55) where "f oooo g \<equiv> \<lambda>x. f ooo (g x)"
+*)
 
 lemma [sepref_fr_rules]:
-  \<open>(uncurry3 (return oooo check_linear_combi_l_pre_err_impl),
-   uncurry3 check_linear_combi_l_pre_err) \<in> uint64_nat_assn\<^sup>k *\<^sub>a bool_assn\<^sup>k *\<^sub>a bool_assn\<^sup>k *\<^sub>a bool_assn\<^sup>k \<rightarrow>\<^sub>a raw_string_assn\<close>
-  unfolding list_assn_pure_conv check_linear_combi_l_pre_err_impl_def
-    check_linear_combi_l_pre_err_def 
+  \<open>(uncurry3 (\<lambda>_ _ _ _. Mreturn 0), uncurry3 check_linear_combi_l_pre_err)
+  \<in> (unat_assn' TYPE(64))\<^sup>k *\<^sub>a bool1_assn\<^sup>k *\<^sub>a bool1_assn\<^sup>k *\<^sub>a bool1_assn\<^sup>k \<rightarrow>\<^sub>a raw_string_assn\<close>
+  unfolding check_linear_combi_l_pre_err_def
   apply sepref_to_hoare
-  apply sep_auto
-  done
+  by (vcg; auto simp: status_pure_reassembly)
 
+(* again - we ignore printing for now
 definition check_linear_combi_l_dom_err_impl :: \<open> _ \<Rightarrow> uint64 \<Rightarrow> string\<close> where
   \<open>check_linear_combi_l_dom_err_impl xs i =
   ''Invalid polynomial '' @ show (nat_of_uint64 i)\<close>
+*)
 
 lemma [sepref_fr_rules]:
-  \<open>(uncurry (return oo (check_linear_combi_l_dom_err_impl)),
-  uncurry (check_linear_combi_l_dom_err)) \<in> poly_assn\<^sup>k *\<^sub>a uint64_nat_assn\<^sup>k \<rightarrow>\<^sub>a raw_string_assn\<close>
-  unfolding list_assn_pure_conv check_linear_combi_l_dom_err_impl_def
-    check_linear_combi_l_dom_err_def
+  \<open>(uncurry (\<lambda>_ _. Mreturn 0), uncurry (check_linear_combi_l_dom_err)) 
+  \<in> poly_assn\<^sup>k *\<^sub>a (unat_assn' TYPE(64))\<^sup>k \<rightarrow>\<^sub>a raw_string_assn\<close>
+  unfolding check_linear_combi_l_dom_err_def
   apply sepref_to_hoare
-  apply sep_auto
-  done
+  by (vcg; auto simp: status_pure_reassembly)
 
+(* same thing here
 definition check_linear_combi_l_mult_err_impl :: \<open> _ \<Rightarrow> _ \<Rightarrow> string\<close> where
   \<open>check_linear_combi_l_mult_err_impl xs ys =
   ''Invalid calculation, found'' @ show xs @ '' instead of '' @ show ys\<close>
+*)
 
 lemma [sepref_fr_rules]:
-  \<open>(uncurry (return oo check_linear_combi_l_mult_err_impl),
-  uncurry check_linear_combi_l_mult_err) \<in> poly_assn\<^sup>k *\<^sub>a poly_assn\<^sup>k \<rightarrow>\<^sub>a raw_string_assn\<close>
-  unfolding list_assn_pure_conv check_linear_combi_l_mult_err_impl_def
-    check_linear_combi_l_mult_err_def
+  \<open>(uncurry (\<lambda>_ _. Mreturn 0), uncurry check_linear_combi_l_mult_err) 
+  \<in> poly_assn\<^sup>k *\<^sub>a poly_assn\<^sup>k \<rightarrow>\<^sub>a raw_string_assn\<close>
+  unfolding check_linear_combi_l_mult_err_def
+  unfolding check_linear_combi_l_dom_err_def
   apply sepref_to_hoare
-  apply sep_auto
-  done
+  by (vcg; auto simp: status_pure_reassembly)
 
+(* Elements of a linear combination *)
+abbreviation \<open>lincomb_assn \<equiv> ol_assn (poly_assn \<times>\<^sub>a (unat_assn' TYPE(64)))\<close>
+(* For now, we have to manually build llvm code to free the list.
+ * TODO: Check if we could use a locale in Owning list to avoid this *)
+definition lincomb_tup_free
+  :: "(8 word node ptr node ptr \<times> (64 word \<times> 64 word \<times> 64 word ptr) \<times> 1 word) node ptr \<times> 64 word \<Rightarrow> unit llM" where [llvm_code]:
+  \<open>lincomb_tup_free \<equiv> \<lambda>(p, n). doM { poly_free p; Mreturn () }\<close>
+lemma lincomb_tup_assn_free[sepref_frame_free_rules]: \<open>MK_FREE (poly_assn \<times>\<^sub>a (unat_assn' TYPE(64))) lincomb_tup_free\<close>
+  unfolding lincomb_tup_free_def
+  using free_thms(2,3) poly_assn_free by blast
+  
+definition \<open>lincomb_free \<equiv> ol_delete lincomb_tup_free\<close>
+lemma lincomb_free_simps[llvm_code]:
+  \<open>lincomb_free l = (if l = null then Mreturn () else doM {
+    n \<leftarrow> ll_load l; lincomb_tup_free (node.val n); ll_free l; lincomb_free (node.next n) })\<close>
+  unfolding lincomb_free_def by (rule ol_delete.simps)
+
+lemmas [llvm_pre_simp] = lincomb_free_def[symmetric]
+lemma lincomb_assn_free[sepref_frame_free_rules]: \<open>MK_FREE lincomb_assn lincomb_free\<close>
+  unfolding lincomb_free_def by (rule ol_assn_free[OF lincomb_tup_assn_free])
+
+text \<open>\<open>hd\<close>/\<open>tl\<close> have no implementation on owning lists (\<open>ol_assn\<close>): \<open>hd\<close> would
+  hand out the element while the list retains it, the same sharing problem as
+  map lookup. The owning replacement is \<^const>\<open>op_list_pop_front\<close>
+  (\<open>ol_pop_front_hnr\<close> in \<open>IICF_Owning_List.thy\<close>: one node visit, ownership of the
+  head moves to the caller, no copy). Since the error branch of
+  \<open>linear_combi_l\<close> keeps \<open>xs\<close> unchanged while the success branches take
+  \<open>tl xs\<close>, the pop-front form re-prepends the popped entry in the (cold) error
+  branch: O(1), and abstractly the identity \<open>hd xs # tl xs = xs\<close>.\<close>
+
+definition linear_combi_l2 where
+  \<open>linear_combi_l2 i A \<V> xs = do {
+    ASSERT(linear_combi_l_pre i A \<V> xs);
+    WHILE\<^sub>T
+      (\<lambda>(p, xs, err). xs \<noteq> [] \<and> \<not>is_cfailed err)
+      (\<lambda>(p, xs, _). do {
+         ASSERT(xs \<noteq> []);
+         ASSERT(vars_llist p \<subseteq> \<V>);
+         let ((q\<^sub>0 :: llist_polynomial, i), xs') = op_list_pop_front xs;
+         if (i \<notin># dom_m A \<or> \<not>(vars_llist q\<^sub>0 \<subseteq> \<V>))
+         then do {
+           err \<leftarrow> check_linear_combi_l_dom_err q\<^sub>0 i;
+           RETURN (p, (q\<^sub>0, i) # xs', error_msg i err)
+         } else do {
+           ASSERT(fmlookup A i \<noteq> None);
+           let r = the (fmlookup A i);
+           ASSERT(vars_llist r \<subseteq> \<V>);
+           if q\<^sub>0 = [([], 1)]
+           then do {
+             pq \<leftarrow> add_poly_l (p, r);
+             RETURN (pq, xs', CSUCCESS)
+           }
+           else do {
+             q \<leftarrow> full_normalize_poly (q\<^sub>0);
+             ASSERT(vars_llist q \<subseteq> \<V>);
+             pq \<leftarrow> mult_poly_full q r;
+             ASSERT(vars_llist pq \<subseteq> \<V>);
+             pq \<leftarrow> add_poly_l (p, pq);
+             RETURN (pq, xs', CSUCCESS)
+          }
+         }
+      })
+     ([], xs, CSUCCESS)
+  }\<close>
+
+lemma linear_combi_l2_linear_combi_l:
+  \<open>linear_combi_l2 i A \<V> xs = linear_combi_l i A \<V> xs\<close>
+proof -
+  have H: \<open>(q\<^sub>0, ia) # tl ys = ys\<close> if \<open>hd ys = (q\<^sub>0, ia)\<close> \<open>ys \<noteq> []\<close>
+    for q\<^sub>0 ia and ys :: \<open>(llist_polynomial \<times> nat) list\<close>
+    using that by (cases ys) auto
+  show ?thesis
+    unfolding linear_combi_l2_def linear_combi_l_def op_list_pop_front_def
+    apply (rule bind_cong[OF refl])
+    apply (rule arg_cong2[where f = \<open>\<lambda>c b. WHILE\<^sub>T c b ([], xs, CSUCCESS)\<close>])
+    subgoal by (rule refl)
+    apply (intro ext)
+    apply (clarsimp split!: prod.splits list.splits simp: H)
+    apply (auto simp: H pw_eq_iff refine_pw_simps)
+    done
+qed
+
+fun vars_of_monom_in where
+  \<open>vars_of_monom_in [] _ = True\<close> |
+  \<open>vars_of_monom_in (x # xs) \<V> \<longleftrightarrow> x \<in> \<V> \<and> vars_of_monom_in xs \<V>\<close>
+
+fun vars_of_poly_in where
+  \<open>vars_of_poly_in [] _ = True\<close> |
+  \<open>vars_of_poly_in ((x, _) # xs) \<V> \<longleftrightarrow> vars_of_monom_in x \<V> \<and> vars_of_poly_in xs \<V>\<close>
+
+lemma vars_of_monom_in_alt_def:
+  \<open>vars_of_monom_in xs \<V> \<longleftrightarrow> set xs \<subseteq> \<V>\<close>
+  by (induction xs)
+   auto
+
+lemma vars_llist_alt_def:
+  \<open>vars_llist xs \<subseteq> \<V> \<longleftrightarrow> vars_of_poly_in xs \<V>\<close>
+  by (induction xs)
+   (auto simp: vars_llist_def vars_of_monom_in_alt_def)
+
+text \<open>The fold-form synthesis of the original AFP (\<open>vars_of_monom_in_alt_def2\<close> +
+  \<open>by sepref\<close>) does not port: \<open>fold\<close> is not a sepref combinator in this
+  framework (monadify stalls on \<open>EVAL $ (\<lambda>x. \<dots>)\<close>), and there is no generic
+  read-only iteration over owning lists anyway. Instead the test is a fused
+  recursive walk in the \<open>poly_eq_impl\<close>/\<open>mnml_eq_impl\<close> ladder style: walk the
+  polynomial spine, per monomial walk the string spine, one hash-set membership
+  per variable (\<open>vars_hs_member_rule\<close>, \<open>String_Assn.thy\<close>), early exit on the
+  first miss. Everything is keep-mode; the set assertion stays folded
+  throughout.\<close>
+
+partial_function (M) vars_of_monom_in_impl ::
+  \<open>8 word os_list hs_impl \<Rightarrow> monom_conc \<Rightarrow> 1 word llM\<close> where
+  \<open>vars_of_monom_in_impl vi p = (if p = null then Mreturn 1
+    else doM {
+      n \<leftarrow> ll_load p;
+      b \<leftarrow> vars_hs_member_impl (node.val n) vi;
+      if to_bool b then vars_of_monom_in_impl vi (node.next n)
+      else Mreturn 0
+    })\<close>
+
+lemmas [llvm_code] = vars_of_monom_in_impl.simps
+
+lemma vars_of_monom_in_impl_rule[vcg_rules]:
+  \<open>llvm_htriple
+    (monom_assn xs p ** vars_hs_assn \<V> vi)
+    (vars_of_monom_in_impl vi p)
+    (\<lambda>r. monom_assn xs p ** vars_hs_assn \<V> vi
+       ** \<upharpoonleft>bool.assn (vars_of_monom_in xs \<V>) r)\<close>
+  unfolding ol_assn_conv
+proof (induction xs arbitrary: p)
+  case Nil
+  show ?case
+    supply [simp] = bool.assn_def
+    apply (subst vars_of_monom_in_impl.simps)
+    by vcg
+next
+  case (Cons e es)
+  note [vcg_rules] = Cons.IH vars_hs_member_rule
+  show ?case
+    supply [simp, named_ss fri_prepare_simps] = ol_seg_cons
+    supply [simp] = bool.assn_def sep_conj_exists
+    apply (subst vars_of_monom_in_impl.simps)
+    apply (cases \<open>p = null\<close>; simp)
+    by vcg
+qed
+
+partial_function (M) vars_of_poly_in_impl ::
+  \<open>8 word os_list hs_impl \<Rightarrow> (monom_conc \<times> sbin_conc \<times> 1 word) os_list \<Rightarrow> 1 word llM\<close> where
+  \<open>vars_of_poly_in_impl vi p = (if p = null then Mreturn 1
+    else doM {
+      n \<leftarrow> ll_load p;
+      b \<leftarrow> vars_of_monom_in_impl vi (fst (node.val n));
+      if to_bool b then vars_of_poly_in_impl vi (node.next n)
+      else Mreturn 0
+    })\<close>
+
+lemmas [llvm_code] = vars_of_poly_in_impl.simps
+
+lemma vars_of_poly_in_impl_rule[vcg_rules]:
+  \<open>llvm_htriple
+    (poly_assn xs p ** vars_hs_assn \<V> vi)
+    (vars_of_poly_in_impl vi p)
+    (\<lambda>r. poly_assn xs p ** vars_hs_assn \<V> vi
+       ** \<upharpoonleft>bool.assn (vars_of_poly_in xs \<V>) r)\<close>
+  unfolding ol_assn_conv
+proof (induction xs arbitrary: p)
+  case Nil
+  show ?case
+    supply [simp] = bool.assn_def
+    apply (subst vars_of_poly_in_impl.simps)
+    by vcg
+next
+  case (Cons e es)
+  note [vcg_rules] = Cons.IH vars_of_monom_in_impl_rule[unfolded ol_assn_conv]
+  show ?case
+    supply [simp, named_ss fri_prepare_simps] = ol_seg_cons
+    supply [simp] = bool.assn_def sep_conj_exists
+    apply (subst vars_of_poly_in_impl.simps)
+    apply (cases \<open>p = null\<close>; cases e; simp)
+    by vcg
+qed
+
+sepref_register vars_of_poly_in
+
+lemma vars_of_poly_in_hnr[sepref_fr_rules]:
+  \<open>(uncurry (\<lambda>pi vi. vars_of_poly_in_impl vi pi), uncurry (RETURN oo vars_of_poly_in))
+    \<in> poly_assn\<^sup>k *\<^sub>a vars_hs_assn\<^sup>k \<rightarrow>\<^sub>a bool1_assn\<close>
+  unfolding bool1_rel_def bool.assn_is_rel[symmetric]
+  apply sepref_to_hoare
+  by vcg
+
+(* Note that we have to destroy lincomb - Check in outer loop if 
+   that could be tolerated by contiuing with tl, otherwise we need
+   to copy the hd out of the list *)
 sepref_definition linear_combi_l_impl
   is \<open>uncurry3 linear_combi_l\<close>
-  :: \<open>uint64_nat_assn\<^sup>k *\<^sub>a polys_assn\<^sup>k *\<^sub>a vars_assn\<^sup>k *\<^sub>a (list_assn (poly_assn \<times>\<^sub>a uint64_nat_assn))\<^sup>k  \<rightarrow>\<^sub>a
-  poly_assn \<times>\<^sub>a (list_assn (poly_assn \<times>\<^sub>a uint64_nat_assn)) \<times>\<^sub>a status_assn raw_string_assn\<close>
-  supply [[goals_limit=1]]
-  unfolding linear_combi_l_def  check_linear_combi_l_def conv_to_is_Nil
-    term_order_rel'_def[symmetric]
-    term_order_rel'_alt_def
-    in_dom_m_lookup_iff
-    fmlookup'_def[symmetric]
-    vars_llist_alt_def is_Nil_def
-  unfolding
-    HOL_list.fold_custom_empty
-  apply (rewrite in \<open>(op_HOL_list_empty, _)\<close> annotate_assn[where A=\<open>poly_assn\<close>])
+  \<comment> \<open>The id \<open>i\<close> is \<open>unat\<close>, not \<open>snat\<close>: inside \<open>linear_combi_l\<close> it is only used in
+    the precondition ASSERT (no operation), but the caller
+    (\<open>check_linear_combi_l\<close>) feeds the \<^emph>\<open>same\<close> id to \<open>op_fmap_contains_key\<close> and
+    \<open>error_msg\<close>, whose keys are \<open>unat\<close> \<comment> \<open>the assertions must agree at the call.\<close>\<close>
+  :: \<open>(unat_assn' TYPE(64))\<^sup>k *\<^sub>a polys_assn\<^sup>k *\<^sub>a vars_hs_assn\<^sup>k *\<^sub>a lincomb_assn\<^sup>d
+       \<rightarrow>\<^sub>a poly_assn \<times>\<^sub>a lincomb_assn \<times>\<^sub>a status_assn raw_string_assn\<close>
+  unfolding linear_combi_l2_linear_combi_l[symmetric]
+  unfolding linear_combi_l2_def
+  unfolding check_linear_combi_l_def
+  unfolding conv_to_is_Nil
+  unfolding term_order_rel'_def[symmetric]
+  unfolding term_order_rel'_alt_def
+  unfolding fmlookup'_def[symmetric]
+  unfolding fold_is_Nil_is_empty
+  unfolding fold_ol_empty
+  unfolding vars_llist_alt_def
   by sepref
 
 definition has_failed :: \<open>bool nres\<close> where
   \<open>has_failed = RES UNIV\<close>
 
-lemma [sepref_fr_rules]:
-  \<open>(uncurry0 (return False), uncurry0 has_failed)\<in>unit_assn\<^sup>k \<rightarrow>\<^sub>a bool_assn\<close>
-  by sepref_to_hoare
-    (sep_auto simp: has_failed_def)
+text \<open>The concrete side never fails spuriously: \<open>Mreturn 0\<close> refines the
+  nondeterministic \<open>RES UNIV\<close> by always choosing \<open>False\<close>.\<close>
 
-declare linear_combi_l_impl.refine[sepref_fr_rules]
-  sepref_register check_linear_combi_l_pre_err
+sepref_register has_failed
+lemma has_failed_hnr[sepref_fr_rules]:
+  \<open>(uncurry0 (Mreturn 0), uncurry0 has_failed) \<in> unit_assn\<^sup>k \<rightarrow>\<^sub>a bool1_assn\<close>
+  unfolding has_failed_def bool1_rel_def bool.assn_is_rel[symmetric]
+  apply sepref_to_hoare
+  by (vcg; auto simp: status_pure_reassembly bool.assn_def refine_pw_simps)
+
+sepref_register check_linear_combi_l_pre_err
+
+text \<open>\<open>linear_combi_l\<close> is \<^emph>\<open>inlined\<close> here rather than called as a registered
+  operation. A registered call fails: \<open>linear_combi_l\<close> returns a triple carrying an
+  \<^emph>\<open>owning\<close> list (\<open>lincomb_assn\<close>), and \<open>sepref_register\<close> gives its \<open>fmap\<close> argument the
+  plain \<open>fmap\<close> interface rather than \<open>f_map\<close>, so the argument-\<open>ID\<close>s never resolve.
+  Inlining sidesteps both, and \<^const>\<open>check_linear_combi_l\<close> itself returns a simple
+  status, so \<^emph>\<open>it\<close> registers cleanly for \<open>check_step\<close> (mirrors the AFP, where
+  \<open>check_addition_l\<close> inlines its loop). The unfold set is
+  \<open>linear_combi_l_impl\<close>'s (pop-front \<open>linear_combi_l2\<close> + loop discipline) plus
+  \<open>check_linear_combi_l\<close>'s own outer control: \<open>has_failed_def[symmetric]\<close> for the
+  \<open>RES UNIV\<close> allocation-failure nondeterminism, \<open>conv_to_is_Nil\<close>/\<open>fold_is_Nil_is_empty\<close>
+  for the \<open>xs = []\<close> tests, \<open>vars_llist_alt_def\<close> for the subset tests. The leftover
+  owning list from the loop is discarded in \<open>check\<close> and freed by \<open>lincomb_assn_free\<close>.\<close>
+
 sepref_definition check_linear_combi_l_impl
   is \<open>uncurry5 check_linear_combi_l\<close>
-  :: \<open>poly_assn\<^sup>k *\<^sub>a polys_assn\<^sup>k *\<^sub>a vars_assn\<^sup>k *\<^sub>a uint64_nat_assn\<^sup>k *\<^sub>a
-        (list_assn (poly_assn \<times>\<^sub>a uint64_nat_assn))\<^sup>k *\<^sub>a poly_assn\<^sup>k  \<rightarrow>\<^sub>a status_assn raw_string_assn\<close>
+  :: \<open>poly_assn\<^sup>k *\<^sub>a polys_assn\<^sup>k *\<^sub>a vars_hs_assn\<^sup>k *\<^sub>a (unat_assn' TYPE(64))\<^sup>k *\<^sub>a
+        lincomb_assn\<^sup>d *\<^sub>a poly_assn\<^sup>k \<rightarrow>\<^sub>a status_assn raw_string_assn\<close>
   supply [[goals_limit=1]]
-  unfolding check_mult_l_def  check_linear_combi_l_def conv_to_is_Nil
-    term_order_rel'_def[symmetric]
-    term_order_rel'_alt_def
-    in_dom_m_lookup_iff
-    fmlookup'_def[symmetric]
-    vars_llist_alt_def is_Nil_def
-    has_failed_def[symmetric]
-   by sepref
+  unfolding check_linear_combi_l_def
+  unfolding linear_combi_l2_linear_combi_l[symmetric]
+  unfolding linear_combi_l2_def
+  unfolding conv_to_is_Nil
+  unfolding term_order_rel'_def[symmetric]
+  unfolding term_order_rel'_alt_def
+  unfolding fmlookup'_def[symmetric]
+  unfolding fold_is_Nil_is_empty
+  unfolding fold_ol_empty
+  unfolding vars_llist_alt_def
+  unfolding has_failed_def[symmetric]
+  by sepref
 
 declare check_linear_combi_l_impl.refine[sepref_fr_rules]
 
@@ -126,16 +345,29 @@ definition check_extension_l2_cond :: \<open>nat \<Rightarrow> _\<close> where
 definition check_extension_l2_cond2 :: \<open>nat \<Rightarrow> _\<close> where
   \<open>check_extension_l2_cond2 i A \<V> v = RETURN (fmlookup' i A = None \<and> v \<notin> \<V>)\<close>
 
+(* TODO: We don't have a refinment target for option types, we need to manually refine this
+   to the bool valued contains test *)
 
 sepref_definition check_extension_l2_cond2_impl
   is \<open>uncurry3 check_extension_l2_cond2\<close>
-    :: \<open>uint64_nat_assn\<^sup>k *\<^sub>a polys_assn\<^sup>k *\<^sub>a vars_assn\<^sup>k *\<^sub>a string_assn\<^sup>k \<rightarrow>\<^sub>a bool_assn\<close>
+    :: \<open>(unat_assn' TYPE(64))\<^sup>k *\<^sub>a polys_assn\<^sup>k *\<^sub>a vars_hs_assn\<^sup>k *\<^sub>a strl_assn\<^sup>k \<rightarrow>\<^sub>a bool1_assn\<close>
   supply [[goals_limit=1]]
   unfolding check_extension_l2_cond2_def
     in_dom_m_lookup_iff
-    fmlookup'_def[symmetric]
     not_not is_None_def
-  by sepref
+  apply sepref_dbg_preproc
+  apply sepref_dbg_cons_init
+  apply sepref_dbg_id
+  apply sepref_dbg_id_keep
+  apply sepref_dbg_monadify
+  apply sepref_dbg_opt_init
+  apply sepref_dbg_trans
+  apply sepref_dbg_opt
+  apply sepref_dbg_cons_solve
+  apply sepref_dbg_cons_solve
+  apply sepref_dbg_cons_solve_cp
+  apply sepref_dbg_constraints
+  oops
 
 lemma check_extension_l2_cond2_check_extension_l2_cond:
   \<open>(uncurry3 check_extension_l2_cond2, uncurry3 check_extension_l2_cond) \<in>
@@ -146,51 +378,49 @@ lemma check_extension_l2_cond2_check_extension_l2_cond:
 lemmas [sepref_fr_rules] =
   check_extension_l2_cond2_impl.refine[FCOMP check_extension_l2_cond2_check_extension_l2_cond]
 
-
+(* Again, we don't do printing for now
 definition check_extension_l_side_cond_err_impl :: \<open>_ \<Rightarrow> _\<close>  where
   \<open>check_extension_l_side_cond_err_impl v r s =
     ''Error while checking side conditions of extensions polynow, var is '' @ show v @
     ''side condition p*p - p = '' @ show s @ '' and should be 0''\<close>
+*)
 term check_extension_l_side_cond_err
 lemma [sepref_fr_rules]:
-  \<open>(uncurry2 (return ooo (check_extension_l_side_cond_err_impl)),
-    uncurry2 (check_extension_l_side_cond_err)) \<in> string_assn\<^sup>k *\<^sub>a poly_assn\<^sup>k *\<^sub>a poly_assn\<^sup>k \<rightarrow>\<^sub>a raw_string_assn\<close>
-   unfolding check_extension_l_side_cond_err_impl_def check_extension_l_side_cond_err_def
-     list_assn_pure_conv
-   apply sepref_to_hoare
-   apply sep_auto
-   done
+  \<open>(uncurry2 (\<lambda>_ _ _. Mreturn 0), uncurry2 (check_extension_l_side_cond_err)) 
+  \<in> strl_assn\<^sup>k *\<^sub>a poly_assn\<^sup>k *\<^sub>a poly_assn\<^sup>k \<rightarrow>\<^sub>a raw_string_assn\<close>
+  unfolding check_extension_l_side_cond_err_def
+  apply sepref_to_hoare
+  by (vcg; auto simp: status_pure_reassembly)
 
+(* No printing for now
 definition check_extension_l_new_var_multiple_err_impl :: \<open>_ \<Rightarrow> _\<close>  where
   \<open>check_extension_l_new_var_multiple_err_impl v p =
     ''Error while checking side conditions of extensions polynow, var is '' @ show v @
     '' but it either appears at least once in the polynomial or another new variable is created '' @
     show p @ '' but should not.''\<close>
+*)
 
 lemma [sepref_fr_rules]:
-  \<open>((uncurry (return oo (check_extension_l_new_var_multiple_err_impl))),
-    uncurry (check_extension_l_new_var_multiple_err)) \<in> string_assn\<^sup>k *\<^sub>a poly_assn\<^sup>k \<rightarrow>\<^sub>a raw_string_assn\<close>
-   unfolding check_extension_l_new_var_multiple_err_impl_def
+  \<open>(uncurry (\<lambda>_ _. Mreturn 0), uncurry (check_extension_l_new_var_multiple_err)) 
+  \<in> strl_assn\<^sup>k *\<^sub>a poly_assn\<^sup>k \<rightarrow>\<^sub>a raw_string_assn\<close>
+  unfolding
      check_extension_l_new_var_multiple_err_def
-     list_assn_pure_conv
-   apply sepref_to_hoare
-   apply sep_auto
-   done
+  apply sepref_to_hoare
+  by (vcg; auto simp: status_pure_reassembly)
 
 sepref_definition check_extension_l_impl
   is \<open>uncurry5 check_extension_l2\<close>
-    :: \<open>poly_assn\<^sup>k *\<^sub>a polys_assn\<^sup>k *\<^sub>a vars_assn\<^sup>k *\<^sub>a uint64_nat_assn\<^sup>k *\<^sub>a
-    string_assn\<^sup>k *\<^sub>a poly_assn\<^sup>k \<rightarrow>\<^sub>a status_assn raw_string_assn\<close>
+    :: \<open>poly_assn\<^sup>k *\<^sub>a polys_assn\<^sup>k *\<^sub>a vars_hs_assn\<^sup>k *\<^sub>a (unat_assn' TYPE(64))\<^sup>k *\<^sub>a
+    strl_assn\<^sup>k *\<^sub>a poly_assn\<^sup>k \<rightarrow>\<^sub>a status_assn raw_string_assn\<close>
   supply [[goals_limit=1]]
   unfolding check_extension_l2_def
     in_dom_m_lookup_iff
-    fmlookup'_def[symmetric]
     not_not is_None_def
     uminus_poly_def[symmetric]
-    HOL_list.fold_custom_empty
     check_extension_l2_cond_def[symmetric]
     vars_llist_alt_def
-  by sepref
+  apply sepref_dbg_keep
+  oops
 
 lemmas [sepref_fr_rules] =
   check_extension_l_impl.refine
@@ -201,16 +431,16 @@ lemma is_Mult_lastI:
 
 sepref_definition check_step_impl
   is \<open>uncurry4 PAC_checker_l_step'\<close>
-  :: \<open>poly_assn\<^sup>k *\<^sub>a (status_assn raw_string_assn)\<^sup>d *\<^sub>a vars_assn\<^sup>d *\<^sub>a polys_assn\<^sup>d *\<^sub>a (pac_step_rel_assn (uint64_nat_assn) poly_assn (string_assn :: string \<Rightarrow> _))\<^sup>d \<rightarrow>\<^sub>a
-    status_assn raw_string_assn \<times>\<^sub>a vars_assn \<times>\<^sub>a polys_assn\<close>
-  supply [[goals_limit=1]] is_Mult_lastI[intro] single_valued_uint64_nat_rel[simp]
+  :: \<open>poly_assn\<^sup>k *\<^sub>a (status_assn raw_string_assn)\<^sup>d *\<^sub>a vars_hs_assn\<^sup>d *\<^sub>a polys_assn\<^sup>d 
+      *\<^sub>a (pac_step_rel_assn (unat_assn' TYPE(64)) poly_assn strl_assn)\<^sup>d \<rightarrow>\<^sub>a
+         status_assn raw_string_assn \<times>\<^sub>a vars_hs_assn \<times>\<^sub>a polys_assn\<close>
   unfolding PAC_checker_l_step_def PAC_checker_l_step'_def
     pac_step.case_eq_if Let_def
      is_success_alt_def[symmetric]
     uminus_poly_def[symmetric]
     HOL_list.fold_custom_empty
-  by sepref
-
+  apply sepref_dbg_keep
+  oops
 
 declare check_step_impl.refine[sepref_fr_rules]
 
@@ -237,16 +467,18 @@ lemma step_rewrite_pure:
   apply (auto simp: pure_def relAPP_def)
   done
 
+(* these most likely won't work with llvm anyways
 lemma safe_epac_step_rel_assn[safe_constraint_rules]:
   \<open>CONSTRAINT is_pure K \<Longrightarrow> CONSTRAINT is_pure V \<Longrightarrow> CONSTRAINT is_pure R \<Longrightarrow>
   CONSTRAINT is_pure (LPAC_Checker.pac_step_rel_assn K V R)\<close>
   by (auto simp: step_rewrite_pure(1)[symmetric] is_pure_conv)
+*)
 
 sepref_definition PAC_checker_l_impl
   is \<open>uncurry4 PAC_checker_l'\<close>
-  :: \<open>poly_assn\<^sup>k *\<^sub>a vars_assn\<^sup>d *\<^sub>a polys_assn\<^sup>d *\<^sub>a (status_assn raw_string_assn)\<^sup>d *\<^sub>a
+  :: \<open>poly_assn\<^sup>k *\<^sub>a vars_hs_assn\<^sup>d *\<^sub>a polys_assn\<^sup>d *\<^sub>a (status_assn raw_string_assn)\<^sup>d *\<^sub>a
        (list_assn (pac_step_rel_assn (uint64_nat_assn) poly_assn string_assn))\<^sup>k \<rightarrow>\<^sub>a
-     status_assn raw_string_assn \<times>\<^sub>a vars_assn \<times>\<^sub>a polys_assn\<close>
+     status_assn raw_string_assn \<times>\<^sub>a vars_hs_assn \<times>\<^sub>a polys_assn\<close>
   supply [[goals_limit=1]] is_Mult_lastI[intro]
   unfolding PAC_checker_l_def is_success_alt_def[symmetric] PAC_checker_l_step_alt_def
     nres_bind_let_law[symmetric] PAC_checker_l'_def
@@ -259,15 +491,17 @@ declare PAC_checker_l_impl.refine[sepref_fr_rules]
 abbreviation polys_assn_input where
   \<open>polys_assn_input \<equiv> iam_fmap_assn nat_assn poly_assn\<close>
 
+(* ignore printing for now
 definition remap_polys_l_dom_err_impl :: \<open>_\<close>  where
   \<open>remap_polys_l_dom_err_impl =
     ''Error during initialisation. Too many polynomials where provided. If this happens,'' @
     ''please report the example to the authors, because something went wrong during '' @
     ''code generation (code generation to arrays is likely to be broken).''\<close>
+*)
 
 lemma [sepref_fr_rules]:
-  \<open>((uncurry0 (return (remap_polys_l_dom_err_impl))),
-    uncurry0 (remap_polys_l_dom_err)) \<in> unit_assn\<^sup>k \<rightarrow>\<^sub>a raw_string_assn\<close>
+  \<open>(uncurry0 (Mreturn 0), uncurry0 (remap_polys_l_dom_err)) 
+  \<in> unit_assn\<^sup>k \<rightarrow>\<^sub>a raw_string_assn\<close>
    unfolding remap_polys_l_dom_err_def
      remap_polys_l_dom_err_def
      list_assn_pure_conv
